intmap overhaul

bin/query/M.ml
@@ -7,16 +7,4 @@ let empty = SM.empty
 let insert = SM.add
 let lookup = SM.find_opt
 let size = SM.cardinal
-let bindings = SM.bindings
-(* 
-let printMap m =
-  SM.iter (fun key value -> Printf.printf "%s -> %d\n" key value) m
- *)
-
-(* let tr_concat xss =
-  let rec aux acc ls =
-    match ls with
-    | [] -> acc
-    | xs :: xss' -> aux (List.rev_append xs acc) xss'
-  in aux [] xss
- *)
+let to_list = SM.bindings
