theory/Util/AssocList.v
@@ -3,35 +3,94 @@ Import ListNotations.
 
 Require Import Games.Util.Dec.
 
-Definition t (K V : Type) : Type :=
-  list (K * V).
+Record t (K V : Type) : Type := {
+  assoc_list : list (K * V);
+  nd_keys : NoDup (map fst assoc_list);
+  }.
 
-Definition empty {K V} : t K V := [].
+Arguments assoc_list {_} {_} _.
+Arguments nd_keys {_} {_} _.
 
-Fixpoint add {K V} `{Discrete K}
-  (k : K) (v : V) (ps : t K V) : t K V :=
+Definition empty {K V} : t K V := {|
+  assoc_list := [];
+  nd_keys := NoDup_nil _;
+  |}.
+
+Fixpoint al_add {K V} `{Discrete K}
+  (k : K) (v : V) (ps : list (K * V)) : list (K * V) :=
   match ps with
   | [] => [(k,v)]
   | (k',v') :: qs =>
     match eq_dec k k' with
     | left _ => (k,v) :: qs
-    | right _ => (k',v') :: add k v qs
+    | right _ => (k',v') :: al_add k v qs
     end
   end.
 
-Fixpoint lookup {K V} `{Discrete K}
-  (k : K) (ps : t K V) : option V :=
+Lemma In_al_add_inv {K V} `{Discrete K} (k : K) (v : V) p m :
+  In p (al_add k v m) -> p = (k, v) \/ In p m.
+Proof.
+  induction m as [|[k' v'] l]; intro pf.
+  - left; destruct pf as [|[]].
+    congruence.
+  - simpl in pf.
+    destruct eq_dec.
+    + subst.
+      destruct pf.
+      * left; congruence.
+      * right; right; auto.
+    + destruct pf as [pf|pf].
+      * right; left; congruence.
+      * apply IHl in pf.
+        destruct pf.
+        -- now left.
+        -- right; now right.
+Qed.
+
+Lemma al_add_NoDup {K V} `{Discrete K} {k} {v} {ps : list (K * V)} :
+  NoDup (map fst ps) ->
+  NoDup (map fst (al_add k v ps)).
+Proof.
+  induction ps as [|[k' v'] l']; intro pf.
+  - constructor; [|constructor].
+    intros [].
+  - simpl in *.
+    destruct eq_dec; simpl.
+    + congruence.
+    + constructor.
+      * intro Hin.
+        rewrite in_map_iff in Hin.
+        destruct Hin as [[k'' v''] [pf1 pf2]].
+        simpl in *; subst.
+        apply In_al_add_inv in pf2.
+        destruct pf2 as [pf2|pf2].
+        -- congruence.
+        -- rewrite NoDup_cons_iff in pf.
+           destruct pf as [pf _].
+           apply pf.
+           apply in_map with (f := fst) in pf2; auto.
+      * apply IHl'.
+        inversion pf; auto.
+Qed.
+
+Definition add {K V} `{Discrete K} (k : K) (v : V) (m : t K V) : t K V := {|
+  assoc_list := al_add k v (assoc_list m);
+  nd_keys := al_add_NoDup (nd_keys m);
+  |}.
+
+Fixpoint al_lookup {K V} `{Discrete K}
+  (k : K) (ps : list (K * V)) : option V :=
   match ps with
   | [] => None
   | (k',v) :: qs =>
     match eq_dec k k' with
     | left _ => Some v
-    | right _ => lookup k qs
+    | right _ => al_lookup k qs
     end
   end.
 
-Definition size {K V} (ps : t K V) : nat :=
-  length ps.
+Definition lookup {K V} `{Discrete K} (k : K) (m : t K V) : option V :=
+  al_lookup k (assoc_list m).
 
 Lemma lookup_empty {K V} `{Discrete K} : forall k,
   lookup k (empty : t K V) = None.
@@ -42,7 +101,8 @@ Qed.
 Lemma lookup_add {K V} `{Discrete K} : forall (k : K) (v : V) m,
   lookup k (add k v m) = Some v.
 Proof.
-  intros k v m.
+  unfold lookup.
+  intros k v [m nd]; simpl; clear nd.
   induction m as [|[k' v'] m'].
   - simpl; now destruct (eq_dec k k).
   - simpl; destruct (eq_dec k k').
@@ -53,7 +113,8 @@ Qed.
 Lemma lookup_add_neq {K V} `{Discrete K} : forall (k k' : K) (v : V) m,
   k <> k' -> lookup k (add k' v m) = lookup k m.
 Proof.
-  intros k k' v m Hkk'.
+  unfold lookup.
+  intros k k' v [m nd] Hkk'; simpl; clear nd.
   induction m as [|[k'' v''] m'].
   - simpl; now destruct (eq_dec k k').
   - simpl; destruct (eq_dec k' k'').
@@ -63,23 +124,53 @@ Proof.
     + simpl; now rewrite IHm'.
 Qed.
 
-Lemma size_empty {K V} : size (empty : t K V) = 0.
+Definition to_list {K V} (m : t K V) : list (K * V) :=
+  assoc_list m.
+
+Lemma to_list_lookup {K V} `{Discrete K} (m : t K V) k v :
+  In (k, v) (to_list m) -> lookup k m = Some v.
 Proof.
-  reflexivity.
+  unfold to_list, lookup.
+  destruct m as [l nd]; simpl.
+  induction l as [|[k' v'] l']; intro pf.
+  - destruct pf.
+  - destruct pf as [pf|pf]; simpl in *.
+    + inversion pf.
+      destruct eq_dec; auto.
+      contradiction.
+    + rewrite NoDup_cons_iff in nd.
+      destruct nd as [nIn nd].
+      destruct eq_dec.
+      * subst; simpl in *.
+        elim nIn.
+        apply in_map with (f := fst) in pf; auto.
+      * apply IHl'; auto.
 Qed.
 
-Lemma size_add {K V} `{Discrete K} : forall (k : K) (v : V) m,
-  size (add k v m) =
-    match lookup k m with
-    | Some _ => size m
-    | None => S (size m)
-    end.
+Lemma lookup_to_list {K V} `{Discrete K} (m : t K V) k v :
+  lookup k m = Some v -> In (k, v) (to_list m).
 Proof.
-  intros k v m.
-  induction m as [|[k' v'] m'].
-  - reflexivity.
-  - simpl.
-    destruct (eq_dec k k').
-    + reflexivity.
-    + simpl; destruct (lookup k m'); auto.
+  unfold to_list, lookup.
+  destruct m as [l nd]; simpl; clear nd.
+  induction l as [|[k' v'] l']; intro pf.
+  - discriminate.
+  - simpl in pf.
+    destruct eq_dec.
+    + left; congruence.
+    + right; apply IHl'; auto.
+Qed.
+
+Lemma to_list_NoDup_keys {K V} `{Discrete K} (m : t K V) :
+  NoDup (map fst (to_list m)).
+Proof.
+  apply m.
+Qed.
+
+Definition size {K V} (m : t K V) : nat :=
+  length (assoc_list m).
+
+Lemma size_to_list {K V} (m : t K V) :
+  size m = length (to_list m).
+Proof.
+  reflexivity.
 Qed.
