theory/Util/OMap.v
@@ -6,6 +6,7 @@ Parameter OM : Type -> Type.
 Parameter empty : forall {X}, OM X.
 Parameter add : forall {X}, int -> X -> OM X -> OM X.
 Parameter lookup : forall {X}, int -> OM X -> option X.
+Parameter to_list : forall {X}, OM X -> list (int * X).
 Parameter size : forall {X}, OM X -> nat.
 
 Axiom lookup_empty : forall {X} str,
@@ -14,24 +15,29 @@ Axiom lookup_add : forall {X} str (x : X) m,
   lookup str (add str x m) = Some x.
 Axiom lookup_add_neq : forall {X} str str' (x : X) m, str <> str' ->
   lookup str (add str' x m) = lookup str m.
-Axiom size_empty : forall {X}, size (empty : OM X) = 0.
-Axiom size_add : forall {X} str (x : X) m,
-  size (add str x m) =
-    match lookup str m with
-    | Some _ => size m
-    | None => S (size m)
-    end.
+
+Axiom to_list_lookup : forall {X} (m : OM X) k v,
+  List.In (k, v) (to_list m) -> lookup k m = Some v.
+Axiom lookup_to_list : forall {X} (m : OM X) k v,
+  lookup k m = Some v -> List.In (k, v) (to_list m).
+Axiom to_list_NoDup_keys : forall {X} (m : OM X),
+  List.NoDup (List.map fst (to_list m)).
+Axiom size_to_list : forall {X} (m : OM X),
+  size m = length (to_list m).
 
 Global Instance OMap : IntMap.IntMap OM := {|
   IntMap.empty := @empty;
   IntMap.add := @add;
   IntMap.lookup := @lookup;
+  IntMap.to_list := @to_list;
   IntMap.size := @size;
   IntMap.lookup_empty := @lookup_empty;
   IntMap.lookup_add := @lookup_add;
   IntMap.lookup_add_neq := @lookup_add_neq;
-  IntMap.size_empty := @size_empty;
-  IntMap.size_add := @size_add
+  IntMap.to_list_lookup := @to_list_lookup;
+  IntMap.lookup_to_list := @lookup_to_list;
+  IntMap.to_list_NoDup_keys := @to_list_NoDup_keys;
+  IntMap.size_to_list := @size_to_list;
   |}.
 
 Require Import Extraction.
@@ -40,5 +46,7 @@ Extraction Language OCaml.
 Extract Constant empty => "M.empty".
 Extract Constant add => "M.insert".
 Extract Constant lookup => "M.lookup".
+Extract Constant to_list => "M.to_list".
 Extract Constant size => "M.size".
+
 Extract Constant OM "'v" => "'v M.t".
